Vector.flush without allocation

ulib/LowStar.Vector.fst
@@ -473,6 +473,39 @@ let insert #a vec v =
     (B.upd vs sz v;
     Vec (sz + 1ul) cap vs)
 
+val shrink:
+  #a:Type -> vec:vector a ->
+  new_size:uint32_t{new_size <= size_of vec} ->
+  Tot (r:vector a{size_of r = new_size})
+let shrink #a vec new_size =
+  Vec new_size (Vec?.cap vec) (Vec?.vs vec)
+
+let rec shift_down (#a:Type) (vec:vector a) (i:uint32_t) (d:uint32_t): HST.ST (rvec:vector a)
+  (requires (fun h0 -> 
+                 live h0 vec /\ 
+                 UInt.size (U32.v i + U32.v d) 32 /\ i + d < size_of vec /\
+                 (i + d) < size_of vec /\
+                 HST.is_eternal_region (frameOf vec)))
+  (ensures (fun h0 rvec h1 -> 
+                live h1 vec /\ live h1 rvec /\ size_of rvec = size_of vec /\
+                modifies (loc_union (loc_vector vec) (loc_vector rvec)) h0 h1 /\
+                frameOf vec = frameOf rvec /\
+                hmap_dom_eq h0 h1 /\
+           S.equal (as_seq h1 rvec)
+              (S.slice (as_seq h0 vec) (U32.v i + 1) (U32.v (size_of vec)))))
+  (decreases (U32.v (size_of vec) - U32.v i))
+= let h0 = HST.get() in
+  if i + d >= size_of vec then vec
+  else begin    
+    assign vec i (index vec (i + d));        
+    let h1 = HST.get() in
+    assume (S.equal (as_seq h1 vec)
+              (S.slice (as_seq h0 vec) (U32.v i + 1) (U32.v (size_of vec))));
+    if (i + d + 1ul >= size_of vec) then vec         
+    else (shift_down vec (i + 1ul) d)
+  end
+
+
 // Flush elements in the vector until the index `i`.
 // It also frees the original allocation and reallocates a smaller space for
 // remaining elements.
@@ -493,20 +526,17 @@ val flush:
       S.equal (as_seq h1 fvec)
               (S.slice (as_seq h0 vec) (U32.v i) (U32.v (size_of vec)))))
 let flush #a vec ia i =
-  let fsz = Vec?.sz vec - i in
-  let asz = if Vec?.sz vec = i then 1ul else fsz in
+  // let fsz = Vec?.sz vec - i in
+  // let asz = if Vec?.sz vec = i then 1ul else fsz in
   let vs = Vec?.vs vec in
-  let fvs = B.malloc (B.frameOf vs) ia asz in
-  B.blit vs i fvs 0ul fsz;
-  B.free vs;
-  Vec fsz asz fvs
-
-val shrink:
-  #a:Type -> vec:vector a ->
-  new_size:uint32_t{new_size <= size_of vec} ->
-  Tot (vector a)
-let shrink #a vec new_size =
-  Vec new_size (Vec?.cap vec) (Vec?.vs vec)
+  // let fvs = B.malloc (B.frameOf vs) ia asz in
+  // B.blit vs i fvs 0ul fsz;
+  // B.free vs;      
+  let h0 = HST.get() in
+  if (i = size_of vec) then
+    Vec 0ul 1ul (B.malloc (B.frameOf vs) ia 1ul)
+  else let shifted = shift_down vec 0ul i in
+    shrink shifted (size_of vec - i)    
   
 
 /// Iteration
